Feb 25

Theorem7.v
@@ -23,7 +23,8 @@ Import Config.
 Import parameters.
 Import Operational_Semantics.
 
-Variable m n:EffVar.
+Definition m:EffVar := effvar "m".
+Definition n:EffVar :=effvar "n".
 Infix " '#-->' " := contract_prop_implication (at level 80).
 Infix " '#\/#' " := contract_prop_disjunction (at level 70).
 Infix " '#/\#' " := contract_prop_conjunction (at level 60).
@@ -38,9 +39,15 @@ Notation " 'ALL'  ":=(contract_untyped_cons) (at level 96).
 
 
 
+(*############################################################# PROVE THIS!!!!!! ######################################################*)
+Notation " '<<' A ',' B ',' C  '>>'  " := (mkSoup_Ing A B C)(at level 10).
+Notation " OP '__' t " := (mkop_cls OP t) (at level 0).
+Notation " A '||' B " := (A +soup+ B). 
+
 Theorem Injection_Help : forall Σ0 Σ ss ii opp s i op τ0 τ oplist σ,
   (Σ0 +soup+  mkSoup_Ing ss ii (mkop_cls opp τ0 :: oplist)) =
   (Σ +soup+  mkSoup_Ing s i (mkop_cls op τ :: σ)) ->
+                              ((Σ0 || << ss,ii+1,oplist>>) = (Σ || << s, i + 1, σ >>)) ->
                                                  σ=oplist /\ τ=τ0 /\ opp=op /\ i=ii /\ s=ss /\ Σ=Σ0.
 Proof. admit. Qed.
 
@@ -48,7 +55,7 @@ Proof. admit. Qed.
 
 Definition Store_Contr (τ:ConsCls):contract_Contract:=
   match τ with
-    |sc =>ALL  m (CONTR: ((PROP: Sameobj m η'') #-->
+    |sc =>ALL  m (CONTR: ((PROP: Sameobj m η'')   #-->
                                          ((PROP: Vis m η'') #\/#
                                           (PROP: Vis η'' m) #\/#
                                           (PROP: Equi m η''))))
@@ -58,13 +65,15 @@ Definition Store_Contr (τ:ConsCls):contract_Contract:=
 Notation " 'Ψ' " := Store_Contr.
 
 
+
 Definition CausCons (Θ:Store)(Ex:Exec):= 
-                                        forall(r: ReplID)(a η:Effect), ((Θ r) η) -> (Ex-A a) -> ((Ex-hbo) a η) -> ((Θ r) a). 
+                                        forall(r: ReplID)(a η:Effect), ((Θ r) η)  -> ((Ex-hbo) a η) -> ((Θ r) a). 
 
 
 Definition Models (Ex:Exec) (cont:contract_Contract) (eff:Effect) : Prop :=
   contract_Eval cont Ex eff (contract_free_number cont).
 Notation " A '|=' B " := (Models A B) (at level 30).
+
 
 
 
@@ -84,9 +93,113 @@ Proof. intros Ex Ex' θ θ' Σ τ s i σ η op.
                 +apply Lemma5 in H1. exact H1. exact HWF.
                 +apply Lemma5 in H0. exact H0. exact HWF.
                
-       -Case"Proof of E'|=Ψτ".
-        inversion H.
-        +admit.
-        +apply Injection_Help in H0. intuition; subst; clear H H1.
-         unfold Models.   cut ( (contract_free_number (Ψ ec)) = 3). intro cut. rewrite cut. *
-         unfold Store_Contr.   compute.   contract_free_number.
+       -Case"Proof of E'|=Ψτ". 
+         inversion H.
+        +SCase"EFFVIS". admit.
+
+        +SCase"[EC]".
+         apply Injection_Help in H0. Focus 2. apply H1.
+         intuition; subst; clear H H1 oplist opcls Σ0; rename ii into i; rename θ' into θ; rename ss into s;rename H7 into H1.
+         inversion H1; subst. compute.
+          intros a Ha; intros b Hb. intros; intuition. 
+         rewrite H9 in H5. intuition.
+         Focus 2.
+         apply CorrectFreshness in H1.
+         compute in H1. apply H1 in H14. inversion H14.
+         remember (E A vis so sameobj) as Ex.
+         assert ((E A' vis' so' sameobj')-hbo a b) as HBO'. 
+         intuition. clear H4.
+
+         assert (Ex-hbo a b). unfold hbo. unfold hbo in HBO'. simpl in HBO'.
+         unfold soo in HBO'. simpl in HBO'. unfold soo.  admit.
+         (*******THIS NEEDS TO BE PROVEN******)
+
+         unfold CausCons in HCausCons.
+         
+         assert ((θ r) a). specialize (HCausCons r a b). apply HCausCons.
+         apply H5.
+         apply H4.
+         specialize (H9 a η). rewrite H9.
+         left. split. apply H8. reflexivity.
+
+
+
+
+         +SCase"[CC]".
+
+
+
+
+
+
+
+
+
+
+
+         
+         
+         specialize (HCausCons r a η). intuition.  apply HCausCons.
+         
+         simpl HCausCons .
+
+
+
+
+
+
+
+
+
+
+
+
+
+
+
+
+
+
+
+
+
+
+
+
+(*
+
+Variable k :Effect.
+
+
+
+
+Definition TestProp : contract_Contract :=  CONTR: (PROP: Sameobj m η'').
+
+Eval compute in contract_Subst (TestProp) k (effvar "m").
+
+
+Definition ηname: string := "η".
+Variable ηsess: SessID.
+Variable ηseq: SeqNo. 
+Variable ηoper: OperName.
+Variable ηval: Value.
+
+Definition Kia : Effect := mkEffect ηname ηsess ηseq ηoper ηval.
+
+Variable kir1 : Exec_A.
+Definition kir4 (i j: Effect) : Prop := True.
+Definition kir2 (i j: Effect) : Prop := True.
+Definition kir3 (i j: Effect) : Prop := True.
+
+
+
+
+                                         
+Definition Ex := (E kir1 kir2 kir3 kir4).
+
+
+Eval compute in contract_free_number(Store_Contr sc).
+Eval compute in Store_Contr sc.
+Eval compute in (Ex |= Ψ sc) Kia.
+
+Eval compute in  contract_free_number (Store_Contr sc).*) 
