parametes_coq.v
@@ -4,6 +4,7 @@ Require Import Coq.Arith.EqNat.
 Require Import Coq.Relations.Relation_Definitions.
 Require Import Coq.Relations.Relation_Operators.
 Require Import Coq.Arith.Compare_dec.
+Require Import Coq.Strings.String.
 
 Module parameters.
   Parameter ReplID :Set.
@@ -11,12 +12,12 @@ Module parameters.
   Parameter OperName : Set.
   Parameter Value : Set.
   Definition SeqNo := nat.
-  Record Effect : Set :=  {sess : SessID; seq : SeqNo; oper : OperName; val:Value}.
+  Record  Effect : Set :=  mkEffect { name:string; sess : SessID; seq : SeqNo; oper : OperName; val:Value}.
   Definition Relation := relation Effect.
   Definition Exec_A := (Ensemble Effect).
   Definition Store := ReplID -> Exec_A.
   Parameter Compute: Exec_A -> OperName -> Value.
-  Parameter dom : Store -> (Ensemble ReplID).
+  Parameter dom : Store -> (Ensemble ReplID).  
 End parameters.
 
 
